DPE with assume global vars

pulse/share/pulse/examples/dice/dpe/DPE.fst
@@ -32,7 +32,7 @@ module U32 = FStar.UInt32
 module PP = PulseCore.Preorder
 module PM = Pulse.Lib.PCMMap
 module FP = Pulse.Lib.PCM.FractionalPreorder
-module M = Pulse.Lib.MutexToken
+module M = Pulse.Lib.Mutex
 module A = Pulse.Lib.Array
 module V = Pulse.Lib.Vec
 module R = Pulse.Lib.Reference
@@ -43,7 +43,7 @@ open PulseCore.Preorder
 open Pulse.Lib.OnRange
 open Pulse.Lib.HashTable.Type
 open Pulse.Lib.HashTable
-open Pulse.Lib.MutexToken
+open Pulse.Lib.Mutex
 open Pulse.Class.PtsTo
 
 // We assume a combinator to run pulse computations for initialization of top-level state, it gets primitive support in extraction
@@ -54,25 +54,56 @@ assume SZ_fits_u32 : SZ.fits_u32
 
 let sid_hash (s:sid_t) : SZ.t = SZ.uint16_to_sizet s
 
-[@@ Rust_const_fn]
+assume val gvar (#a:Type0) (p:a -> slprop) : Type0
+//
+// TODO: add a duplicable precondition to mk_gvar
+//
+assume val mk_gvar #a #p (init:unit -> stt a emp p) : gvar p
+assume val read_gvar_ghost (#a:Type0) (#p:a -> slprop) (x:gvar p) : GTot a
+assume val read_gvar #a #p (x:gvar p)
+  : stt a emp (fun r -> p r ** pure (r == read_gvar_ghost x))
 
+let gvar_p : (gref & mutex (option st)) -> slprop =
+  fun x -> mutex_live (snd x) (dpe_inv (fst x))
+
+[@@ Rust_const_fn]
 fn initialize_global_state ()
   requires emp
-  returns b:(r:gref & mutex (dpe_inv r))
-  ensures emp
+  returns x:(gref & mutex (option st))
+  ensures gvar_p x
 {
   let r = ghost_alloc #_ #pcm all_sids_unused;
   with _v. rewrite (ghost_pcm_pts_to r (G.reveal (G.hide _v))) as
                    (ghost_pcm_pts_to r _v);
   fold (dpe_inv r None);
   let m = new_mutex (dpe_inv r) None;
-  ((| r, m |) <: (r:gref & mutex (dpe_inv r)))
+  let x = r, m;
+  rewrite (mutex_live m (dpe_inv r)) as
+          (gvar_p x);
+  x
 }
 
+let gst : gvar #(gref & mutex (option st)) (fun x -> gvar_p x) = mk_gvar initialize_global_state
 
-let gst : (r:gref & mutex (dpe_inv r)) = run_stt (initialize_global_state ())
+let trace_ref = fst (read_gvar_ghost gst)
 
-let trace_ref = dfst gst
+fn unpack_gst ()
+  requires emp
+  returns m:mutex (option st)
+  ensures mutex_live m (dpe_inv trace_ref) ** pure (m == snd (read_gvar_ghost gst))
+{
+    let r = read_gvar gst;
+    let m = snd r;
+    rewrite (gvar_p r) as (mutex_live m (dpe_inv trace_ref));
+    m
+}
+
+fn pack_gst (m:mutex (option st))
+  requires mutex_live m (dpe_inv trace_ref) ** pure (m == snd (read_gvar_ghost gst))
+  ensures emp
+{
+    drop_ (mutex_live m (dpe_inv trace_ref))
+}
 
 //
 // DPE API implementation
@@ -377,26 +408,25 @@ fn maybe_mk_session_tbl (sopt:option st)
 
 
 
-ghost
-fn to_dpe_inv_trace_ref (#s:option st) ()
-  requires dpe_inv (Mkdtuple2?._1 gst) s
-  ensures dpe_inv trace_ref s
-{
-  rewrite (dpe_inv (Mkdtuple2?._1 gst) s) as
-          (dpe_inv trace_ref s)
-}
+// ghost
+// fn to_dpe_inv_trace_ref (#s:option st) ()
+//   requires dpe_inv (fst (read_gvar_ghost gst)) s
+//   ensures dpe_inv trace_ref s
+// {
+//   rewrite (dpe_inv (Mkdtuple2?._1 gst) s) as
+//           (dpe_inv trace_ref s)
+// }
 
 
 
-ghost
-fn from_dpe_inv_trace_ref (#s:option st) ()
-  requires dpe_inv trace_ref s
-  ensures dpe_inv (Mkdtuple2?._1 gst) s
-{
-  rewrite (dpe_inv trace_ref s) as
-          (dpe_inv (Mkdtuple2?._1 gst) s)
-}
-
+// ghost
+// fn from_dpe_inv_trace_ref (#s:option st) ()
+//   requires dpe_inv trace_ref s
+//   ensures dpe_inv (Mkdtuple2?._1 gst) s
+// {
+//   rewrite (dpe_inv trace_ref s) as
+//           (dpe_inv (Mkdtuple2?._1 gst) s)
+// }
 
 
 fn open_session ()
@@ -404,8 +434,8 @@ fn open_session ()
   returns r:(option sid_t)
   ensures open_session_client_perm r
 {
-  let mg = M.lock (dsnd gst);
-  to_dpe_inv_trace_ref ();
+  let m = unpack_gst ();
+  let mg = M.lock m;
 
   let sopt = M.replace #(option st) mg None;
 
@@ -418,15 +448,14 @@ fn open_session ()
     snd ret as sid_opt;
   mg := Some s;
 
-  from_dpe_inv_trace_ref ();
-  M.unlock (dsnd gst) mg;
+  M.unlock m mg;
+  pack_gst m;
   
   sid_opt
 }
 
 
 [@@allow_ambiguous]
-
 ghost
 fn gather_sid_pts_to (sid:sid_t) (#t0 #t1:trace)
   requires sid_pts_to trace_ref sid t0 **
@@ -504,8 +533,8 @@ fn replace_session
   ensures session_state_related r (current_state t) **
           sid_pts_to trace_ref sid (next_trace t gsst)
 {
-  let mg = M.lock (dsnd gst);
-  to_dpe_inv_trace_ref ();
+  let m = unpack_gst ();
+  let mg = M.lock m;
 
   let sopt = M.replace mg None;
   match sopt {
@@ -572,8 +601,8 @@ fn replace_session
             fold (dpe_inv trace_ref (Some s));
             mg := Some s;
 
-            from_dpe_inv_trace_ref ();
-            M.unlock (dsnd gst) mg;
+            M.unlock m mg;
+            pack_gst m;
 
             st
           }
